WIP

src/tlogic/IndexedInvariants.v
@@ -428,33 +428,362 @@ Section WSATS.
 
 End WSATS.
 
+Notation coPsets := (gmap index coPset).
+
 Section OWNES.
 
   Context `{Σ : GRA.t}.
   Context `{@GRA.inG (index ==> CoPset.t)%ra Σ}.
 
-  Definition OwnE_auth_black (Es : gmap index coPset) : (index ==> CoPset.t)%ra :=
+  Definition OwnE_auth_black (Es : coPsets) : (index ==> CoPset.t)%ra :=
     fun n => match Es !! n with
           | Some _ => ε
           | None => (Some ⊤)
           end.
-  (* Definition OwnE_auth_black (X : gset index) : (index ==> CoPset.t)%ra := *)
-  (*   fun n => if (gset_elem_of_dec n X) *)
-  (*         then ε *)
-  (*         else (Some ⊤). *)
 
-  Definition OwnE_auth (Es : gmap index coPset) := OwnM (OwnE_auth_black Es).
-  (* Definition OwnE_auth (X : gset index) := OwnM (OwnE_auth_black X). *)
-(* gset_dom: *)
-  (*   ∀ (K : Type) (EqDecision0 : EqDecision K) (H : Countable K) (A : Type), Dom (gmap K A) (gset K) *)
+  Definition OwnE_auth (Es : coPsets) := OwnM (OwnE_auth_black Es).
 
-  Definition OwnE_satall (Es : gmap index coPset) := ([∗ map] n ↦ E ∈ Es, OwnE n E)%I.
+  Definition OwnE_satall (Es : coPsets) := ([∗ map] n ↦ E ∈ Es, OwnE n E)%I.
 
-  Definition OwnEs (Es : gmap index coPset) := (OwnE_auth Es ∗ OwnE_satall Es)%I.
+  Definition OwnEs (Es : coPsets) := (OwnE_auth Es ∗ OwnE_satall Es)%I.
+
+  Definition OwnEs_top (Es : coPsets) : Prop := map_Forall (fun _ E => E = ⊤) Es.
+
+  Lemma OwnEs_alloc Es n (NIN : Es !! n = None) :
+    OwnEs Es ⊢ |==> OwnEs (<[n := ⊤]>Es).
+  Proof.
+    iIntros "[AUTH SAT]". unfold OwnE_auth, OwnE_satall.
+    remember (<[n := ⊤]> Es) as Es'.
+    assert (URA.updatable
+              (OwnE_auth_black Es)
+              ((OwnE_auth_black Es')
+                 ⋅
+                 (maps_to_res n (Some ⊤)))).
+    { apply pointwise_updatable. i.
+      unfold OwnE_auth_black, maps_to_res. unfold URA.add. unseal "ra". ss. subst.
+      destruct (excluded_middle_informative (a = n)).
+      - subst a. des_ifs.
+        2:{ exfalso. setoid_rewrite lookup_insert in Heq0. inv Heq0. }
+        rewrite URA.unit_idl. reflexivity.
+      - rewrite lookup_insert_ne; auto. rewrite URA.unit_id. reflexivity.
+    }
+    iMod (OwnM_Upd H0 with "AUTH") as "[AUTH NEW]". clear H0.
+    iModIntro. iFrame. unfold OwnE_satall. subst. iApply big_sepM_insert; auto. iFrame.
+  Qed.
+
+  Lemma OwnEs_acc_in Es n E (IN : Es !! n = Some E) :
+    OwnEs Es ⊢ OwnE n E ∗ OwnEs (<[n := ∅]>Es).
+  Proof.
+    iIntros "[AUTH SAT]". unfold OwnE_satall.
+    iAssert (OwnE n E ∗ ([∗ map] n0↦E0 ∈ delete n Es, OwnE n0 E0))%I with "[SAT]" as "[EN SAT]".
+    { iApply big_sepM_delete; auto. }
+    iPoseProof (OwnM_persistently with "EN") as "#EN2". ss.
+    iAssert ([∗ map] n0↦E0 ∈ <[n := ∅]>Es, OwnE n0 E0)%I with "[SAT]" as "SAT".
+    { iApply big_sepM_insert_delete. iFrame. iApply (OwnM_extends with "EN2").
+      unfold maps_to_res. clear. exists ε. rewrite URA.unit_id. extensionalities a. des_ifs.
+    }
+    iFrame. iClear "EN2".
+    iApply (OwnM_extends with "AUTH"). exists ε. rewrite URA.unit_id. extensionalities a.
+    unfold OwnE_auth_black. destruct (Nat.eqb_spec a n).
+    - subst. rewrite lookup_insert. rewrite IN. auto.
+    - rewrite lookup_insert_ne; auto.
+  Qed.
+
+  Lemma OwnEs_acc_new Es n (NIN : Es !! n = None) :
+    OwnEs Es ⊢ |==> OwnE n ⊤ ∗ OwnEs (<[n := ∅]>Es).
+  Proof.
+    iIntros "ENS". iMod (OwnEs_alloc with "ENS") as "ENS". eauto.
+    iModIntro.
+    assert (<[n:=∅]> Es = <[n:=∅]> (<[n:=⊤]> Es)).
+    { rewrite insert_insert. auto. }
+    rewrite H0. iApply OwnEs_acc_in.
+    - rewrite lookup_insert. auto.
+    - iFrame.
+  Qed.
+
+  Lemma OwnEs_union Es n E1 E2 :
+    OwnEs (<[n:=E1]> Es) ∗ OwnE n E2 ⊢ OwnEs (<[n:=E1 ∪ E2]> Es).
+  Proof.
+    iIntros "[[AUTH SAT] EN]". unfold OwnEs. iSplitL "AUTH".
+    { iApply (OwnM_extends with "AUTH"). exists ε. rewrite URA.unit_id. extensionalities a.
+      unfold OwnE_auth_black. destruct (Nat.eqb_spec a n).
+      - subst. rewrite ! lookup_insert. auto.
+      - rewrite ! lookup_insert_ne; auto.
+    }
+    iApply big_sepM_insert_delete.
+    iAssert (OwnE n E1 ∗ (OwnE_satall (delete n (<[n:=E1]> Es))))%I with "[SAT]" as "[EN' SAT]".
+    { iApply big_sepM_delete.
+      - apply lookup_insert.
+      - iFrame.
+    }
+    assert ((delete n (<[n:=E1]> Es)) = delete n Es).
+    { rewrite delete_insert_delete. auto. }
+    rewrite H0. iFrame. iApply OwnE_union. iFrame.
+  Qed.
+
+
+  Definition lookup_def (Es : coPsets) (n : nat) : coPset := default ⊤ (Es !! n).
+
+  Definition subseteq_def (Es : coPsets) (n : nat) (E : coPset) : Prop :=
+    match Es !! n with | Some E' => E ⊆ E' | None => True end.
+
+  Definition insert_def (Es : coPsets) (n : nat) : coPsets :=
+    match Es !! n with | Some E => Es | None => <[n:=⊤]> Es end.
+
+  Lemma OwnEs_free Es n :
+    Es !! n = None -> OwnEs (<[n:=⊤]>Es) ⊢ |==> OwnEs Es.
+  Proof.
+    iIntros (NIN) "ENS". iPoseProof (OwnEs_acc_in with "ENS") as "[EN ENS]". apply lookup_insert.
+    rewrite insert_insert. unfold OwnEs. iDestruct "ENS" as "[AUTH SAT]".
+    iSplitL "EN AUTH".
+    - unfold OwnE_auth, OwnE. iCombine "EN AUTH" as "AUTH".
+      assert (URA.updatable
+                ((@maps_to_res index CoPset.t n (Some ⊤))
+                   ⋅
+                   OwnE_auth_black (<[n:=∅]> Es))
+                (OwnE_auth_black Es)).
+      { apply pointwise_updatable. i.
+        unfold OwnE_auth_black, maps_to_res. unfold URA.add. unseal "ra". ss.
+        destruct (excluded_middle_informative (a = n)).
+        - subst a. rewrite lookup_insert. rewrite NIN.
+          rewrite URA.unit_id. reflexivity.
+        - rewrite lookup_insert_ne; auto. rewrite URA.unit_idl. reflexivity.
+      }
+      iMod (OwnM_Upd H0 with "AUTH") as "AUTH". iModIntro. iFrame.
+    - unfold OwnE_satall. iModIntro.
+      iPoseProof (big_sepM_insert with "SAT") as "[_ SAT]"; auto.
+  Qed.
+
+  Lemma OwnEs_lookup_def Es n :
+    OwnEs Es ⊢ |==> OwnEs (<[n := lookup_def Es n]>Es).
+  Proof.
+    iIntros "ENS". unfold lookup_def, default. des_ifs; ss.
+    - rewrite insert_id; auto.
+    - iMod (OwnEs_alloc with "ENS") as "ENS"; eauto.
+  Qed.
 
 End OWNES.
 
-TODO
+Section FANCY_UPDATE.
+
+  Context `{Σ : GRA.t}.
+  Context `{Vars : index -> Type}.
+  Context `{Invs : @IInvSet Σ Vars}.
+  Context `{@GRA.inG (index ==> CoPset.t)%ra Σ}.
+  Context `{@GRA.inG (index ==> Gset.t)%ra Σ}.
+  Context `{@GRA.inG (IInvSetRA Vars) Σ}.
+
+  Definition inv (n : index) (N : namespace) P :=
+    (∃ p, ∃ i, ⌜prop n p = P⌝ ∧ ⌜i ∈ (↑N : coPset)⌝ ∧ OwnI n i p)%I.
+
+  Definition FUpd (A : iProp) (Es1 Es2 : coPsets) (P : iProp) : iProp :=
+    A ∗ wsats ∗ OwnEs Es1 -∗ #=> (A ∗ wsats ∗ OwnEs Es2 ∗ P).
+
+
+  Lemma FUpd_alloc A Es n N P `{hasP : @IInvIn Σ Vars Invs n P} :
+    P ⊢ FUpd A Es Es (inv n N P).
+  Proof.
+    destruct hasP as [p HE]. subst. iIntros "P (A & WSAT & EN)".
+    iMod (wsats_OwnI_alloc n p (fun i => i ∈ ↑N) with "[WSAT P]") as "[I WSAT]".
+    - i. des_ifs. apply iris.base_logic.lib.invariants.fresh_inv_name.
+    - iFrame.
+    - iModIntro. iFrame. iDestruct "I" as "[% I]". iExists p, i. iFrame. ss.
+  Qed.
+
+  Lemma FUpd_open_aux A Es n N E (INE : Es !! n = Some E) (IN : ↑N ⊆ E) P :
+    inv n N P ⊢ FUpd A Es (<[n := E∖↑N]> Es) (P ∗ (P -∗ FUpd A (<[n := E∖↑N]> Es) Es emp)).
+  Proof.
+    iIntros "[% [% (%HP & %iN & #HI)]] (A & WSAT & ENS)". subst.
+    iPoseProof ((OwnEs_acc_in _ _ _ INE) with "ENS") as "[EN ENS]".
+    iAssert (OwnE n (E ∖ ↑N) ∗ OwnE n (↑N ∖ {[i]}) ∗ OwnE n {[i]})%I with "[EN]" as "(EN1 & EN2 & EN3)".
+    { iApply bi.sep_mono_r.
+      { apply OwnE_disjoint. set_solver. }
+      iApply OwnE_disjoint.
+      { set_solver. }
+      replace (E ∖ ↑N ∪ (↑N ∖ {[i]} ∪ {[i]})) with E.
+      - iFrame.
+      - transitivity ({[i]} ∪ ↑N ∖ {[i]} ∪ E ∖ ↑N).
+        + rewrite <- union_difference_singleton_L; ss. eapply union_difference_L; ss.
+        + rewrite union_comm_L. f_equal. rewrite union_comm_L. ss.
+    }
+    iMod (wsats_OwnI_open n i p with "[HI WSAT EN3]") as "(P & WSAT & DIS)".
+    { iFrame. auto. }
+    iModIntro. iFrame. iPoseProof (OwnEs_union with "[ENS EN1]") as "ENS". iFrame.
+    replace (∅ ∪ E ∖ ↑N) with (E ∖ ↑N). 2: set_solver.
+    iFrame. iIntros "P (A & WSAT & EN1)".
+    iMod (wsats_OwnI_close n i p with "[HI WSAT P DIS]") as "(WSAT & EN3)".
+    { iFrame. auto. }
+    iModIntro. iFrame. iSplit; auto.
+    iPoseProof (OwnE_union with "[EN2 EN3]") as "EN2". iFrame.
+    rewrite <- union_difference_singleton_L; ss.
+    iPoseProof (OwnEs_union with "[EN1 EN2]") as "ENS". iFrame.
+    rewrite insert_id. iFrame. rewrite INE. f_equal.
+    rewrite difference_union_L. set_solver.
+  Qed.
+
+  Lemma FUpd_open A Es n N (IN : subseteq_def Es n (↑N)) P :
+    inv n N P ⊢
+        FUpd A Es (<[n := (lookup_def Es n)∖↑N]> Es) (P ∗ (P -∗ FUpd A (<[n := (lookup_def Es n)∖↑N]> Es) (insert_def Es n) emp)).
+  Proof.
+    iIntros "[% [% (%HP & %iN & #HI)]] (A & WSAT & ENS)". subst.
+    unfold lookup_def, subseteq_def, insert_def in *. destruct (Es !! n) eqn:CASES; ss.
+    - iApply FUpd_open_aux; auto. unfold inv; auto. iFrame.
+    - iMod (OwnEs_alloc _ _ CASES with "ENS") as "ENS". remember (<[n:=⊤]> Es) as Es'.
+      replace (<[n:=⊤ ∖ ↑N]> Es) with (<[n:=⊤ ∖ ↑N]> Es').
+      2:{ subst. rewrite insert_insert. auto. }
+      iApply FUpd_open_aux; auto.
+      { subst. apply lookup_insert. }
+      unfold inv; auto. iFrame.
+  Qed.
+
+  Lemma FUpd_intro A Es P :
+    #=> P ⊢ FUpd A Es Es P.
+  Proof.
+    iIntros "P H". iMod "P". iModIntro. iFrame. iFrame.
+  Qed.
+
+  Lemma FUpd_mask_frame A Es1 Es2 E P n :
+    (lookup_def Es1 n) ## E ->
+    FUpd A Es1 Es2 P ⊢ FUpd A (<[n := (lookup_def Es1 n) ∪ E]>Es1) (<[n := (lookup_def Es2 n) ∪ E]>Es2) P.
+  Proof.
+    rewrite /FUpd. iIntros (D) "H (A & WSAT & ENS)".
+    iPoseProof ((OwnEs_acc_in _ n) with "ENS") as "[EN ENS]". apply lookup_insert.
+    iPoseProof (OwnE_disjoint _ _ _ D with "EN") as "[EN1 EN]".
+    iPoseProof (OwnEs_union with "[ENS EN1]") as "ENS". iFrame.
+    replace (∅ ∪ lookup_def Es1 n) with (lookup_def Es1 n) by set_solver.
+    destruct (coPset_equiv_dec E ∅); cycle 1.
+    { unfold lookup_def, default in D. des_ifs; ss.
+      2:{ exfalso. set_solver. }
+      rewrite insert_insert. rewrite (insert_id Es1).
+      2:{ unfold lookup_def, default. rewrite Heq. ss. }
+      iPoseProof ("H" with "[A WSAT ENS]") as ">(A & WSAT & ENS2 & P)". iFrame.
+      destruct (Es2 !! n) eqn:CASES.
+      2:{ iMod ((OwnEs_acc_new _ _ CASES) with "ENS2") as "[EN2 _]".
+          iPoseProof (OwnE_exploit with "[EN EN2]") as "%DIS". iFrame.
+          set_solver.
+      }
+      unfold lookup_def. rewrite CASES. ss.
+      iPoseProof ((OwnEs_acc_in _ _ _ CASES) with "ENS2") as "[EN2 ENS]".
+      iPoseProof (OwnE_union with "[EN EN2]") as "EN". iFrame.
+      iPoseProof (OwnEs_union with "[ENS EN]") as "ENS". iFrame.
+      replace (∅ ∪ (c0 ∪ E)) with (c0 ∪ E) by set_solver.
+      iModIntro. iFrame.
+    }
+    { replace (lookup_def Es1 n ∪ E) with (lookup_def Es1 n) by set_solver.
+      replace (lookup_def Es2 n ∪ E) with (lookup_def Es2 n) by set_solver.
+      rewrite insert_insert.
+      destruct (Es1 !! n) eqn:CASES.
+      - rewrite (insert_id Es1).
+        2:{ unfold lookup_def, default. rewrite CASES. ss. }
+        iPoseProof ("H" with "[A WSAT ENS]") as ">(A & WSAT & ENS2 & P)". iFrame.
+        iMod (OwnEs_lookup_def with "ENS2") as "ENS2". iModIntro. iFrame.
+      - replace (lookup_def Es1 n) with (⊤ : coPset).
+        2:{ unfold lookup_def, default. rewrite CASES. ss. }
+        iMod ((OwnEs_free _ _ CASES) with "ENS") as "ENS".
+        iPoseProof ("H" with "[A WSAT ENS]") as ">(A & WSAT & ENS2 & P)". iFrame.
+        iMod (OwnEs_lookup_def with "ENS2") as "ENS2". iModIntro. iFrame.
+    }
+  Qed.
+
+  TODO
+
+  Lemma FUpd_intro_mask A E1 E2 P :
+    E2 ⊆ E1 -> FUpd A E1 E1 P ⊢ FUpd A E1 E2 (FUpd A E2 E1 P).
+  Proof.
+    rewrite /FUpd. iIntros (HE) "H (A & WSAT & EN)".
+    iPoseProof ("H" with "[A WSAT EN]") as ">(A & WSAT & EN & P)". iFrame.
+    iModIntro.
+    rewrite (union_difference_L _ _ HE).
+    iPoseProof (OwnE_disjoint _ _ _ with "EN") as "[EN1 EN]".
+    { set_solver. }
+    iFrame. iIntros "(A & WSAT & EN2)". iModIntro. iFrame.
+    iApply OwnE_union. iFrame.
+  Qed.
+
+  Lemma FUpd_mask_mono A E1 E2 P :
+    E1 ⊆ E2 -> FUpd A E1 E1 P ⊢ FUpd A E2 E2 P.
+  Proof.
+    i. replace E2 with (E1 ∪ E2 ∖ E1).
+    - eapply FUpd_mask_frame. set_solver.
+    - symmetry. eapply leibniz_equiv. eapply union_difference. ss.
+  Qed.
+
+  Global Instance from_modal_FUpd A E P :
+    FromModal True modality_id (FUpd A E E P) (FUpd A E E P) P.
+  Proof.
+    rewrite /FromModal /= /FUpd. iIntros. iModIntro. iFrame. iFrame.
+  Qed.
+
+  Global Instance from_modal_FUpd_general A E1 E2 P :
+    FromModal (E2 ⊆ E1) modality_id P (FUpd A E1 E2 P) P.
+  Proof.
+    rewrite /FromModal /FUpd. ss.
+    iIntros (HE) "P (A & WSAT & EN)". iModIntro. iFrame.
+    iPoseProof ((OwnE_subset _ _ _ HE) with "EN") as "[EN1 _]". iFrame.
+  Qed.
+
+  Global Instance from_modal_FUpd_wrong_mask A E1 E2 P :
+    FromModal (pm_error "Only non-mask-changing update modalities can be introduced directly.
+Use [FUpd_mask_frame] and [FUpd_intro_mask]")
+              modality_id (FUpd A E1 E2 P) (FUpd A E1 E2 P) P | 100.
+  Proof.
+    intros [].
+  Qed.
+
+  Global Instance elim_modal_bupd_FUpd p A E1 E2 P Q :
+    ElimModal True p false (|==> P) P (FUpd A E1 E2 Q) (FUpd A E1 E2 Q) | 10.
+  Proof.
+    rewrite /ElimModal bi.intuitionistically_if_elim /FUpd.
+    iIntros (_) "[P K] I". iMod "P". iApply ("K" with "P"). iFrame.
+  Qed.
+
+  Global Instance elim_modal_FUpd_FUpd p A E1 E2 E3 P Q :
+    ElimModal True p false (FUpd A E1 E2 P) P (FUpd A E1 E3 Q) (FUpd A E2 E3 Q).
+  Proof.
+    rewrite /ElimModal bi.intuitionistically_if_elim /FUpd.
+    iIntros (_) "[P K] I". iMod ("P" with "I") as "(A & WSAT & EN & P)".
+    iApply ("K" with "P"). iFrame.
+  Qed.
+
+  Global Instance elim_modal_FUpd_FUpd_general p A E0 E1 E2 E3 P Q :
+    ElimModal (E0 ⊆ E2) p false (FUpd A E0 E1 P) P (FUpd A E2 E3 Q) (FUpd A (E1 ∪ (E2 ∖ E0)) E3 Q) | 10.
+  Proof.
+    rewrite /ElimModal bi.intuitionistically_if_elim. ss.
+    iIntros (HE) "[M K]".
+    iPoseProof (FUpd_mask_frame _ _ _ (E2 ∖ E0) with "M") as "M".
+    { set_solver. }
+    replace (E0 ∪ E2 ∖ E0) with E2 by (eapply union_difference_L; ss).
+    iMod "M". iPoseProof ("K" with "M") as "M". ss.
+  Qed.
+
+  Global Instance elim_acc_FUpd {X : Type} A E1 E2 E (α β : X -> iProp) (mγ : X -> option iProp) (Q : iProp) :
+    ElimAcc True (FUpd A E1 E2) (FUpd A E2 E1) α β mγ (FUpd A E1 E Q) (fun x : X => ((FUpd A E2 E2 (β x)) ∗ (mγ x -∗? FUpd A E1 E Q))%I).
+  Proof.
+    iIntros (_) "Hinner >[% [Hα Hclose]]".
+    iPoseProof ("Hinner" with "Hα") as "[>Hβ Hfin]".
+    iPoseProof ("Hclose" with "Hβ") as ">Hγ".
+    iApply "Hfin". iFrame.
+  Qed.
+
+  Global Instance into_acc_FUpd_inv A E N P :
+    IntoAcc (inv N P) (↑N ⊆ E) True (FUpd A E (E ∖ ↑N)) (FUpd A (E ∖ ↑N) E) (fun _ : () => P) (fun _ : () => P) (fun _ : () => None).
+  Proof.
+    rewrite /IntoAcc. iIntros (iE) "INV _". rewrite /accessor.
+    iPoseProof (FUpd_open _ _ _ iE with "INV") as ">[open close]".
+    iModIntro. iExists tt. iFrame.
+  Qed.
+
+  Global Instance elim_modal_iupd_FUpd p A E1 E2 P Q :
+    ElimModal True p false (#=(A)=> P) P (FUpd A E1 E2 Q) (FUpd A E1 E2 Q) | 10.
+  Proof.
+    rewrite /ElimModal bi.intuitionistically_if_elim /FUpd.
+    iIntros (_) "[P K] [A I]".
+    iMod ("P" with "A") as "[A P]". iApply ("K" with "P"). iFrame.
+  Qed.
+
+End FANCY_UPDATE.
+
+Global Opaque FUpd.
 
 Section FANCY_UPDATE.
 
